crates/utils/intrinsics/src/avx2.rs
@@ -801,3 +801,12 @@ pub fn mm_aesenclast_si128(a: Vec128, b: Vec128) -> Vec128 {
 pub fn mm_aeskeygenassist_si128<const RCON: i32>(a: Vec128) -> Vec128 {
     unsafe { _mm_aeskeygenassist_si128(a, RCON) }
 }
+
+#[inline(always)]
+pub fn get_lane_u64(vec: Vec256, lane: usize) -> u64 {
+    let mut tmp = [0u64; 4];
+    mm256_storeu_si256_u8(unsafe {
+        core::slice::from_raw_parts_mut(tmp.as_mut_ptr() as *mut u8, 32)
+    }, vec);
+    tmp[lane]
+}
